Validator/Hedge/Elem.lean
@@ -1,0 +1,191 @@
+import Validator.Std.List
+
+import Validator.Regex.Regex
+import Validator.Hedge.Grammar
+
+namespace Hedge.Elem
+
+theorem decreasing_or_l {α: Type} {σ: Type} [SizeOf σ] (r1 r2: Regex σ) (xs: Hedge α):
+  Prod.Lex
+    (fun a₁ a₂ => sizeOf a₁ < sizeOf a₂)
+    (fun a₁ a₂ => sizeOf a₁ < sizeOf a₂)
+    (xs, r1)
+    (xs, Regex.or r1 r2) := by
+  apply Prod.Lex.right
+  simp +arith only [Regex.or.sizeOf_spec]
+
+theorem decreasing_or_r {α: Type} {σ: Type} [SizeOf σ] (r1 r2: Regex σ) (xs: Hedge α):
+  Prod.Lex
+    (fun a₁ a₂ => sizeOf a₁ < sizeOf a₂)
+    (fun a₁ a₂ => sizeOf a₁ < sizeOf a₂)
+    (xs, r2)
+    (xs, Regex.or r1 r2) := by
+  apply Prod.Lex.right
+  simp +arith only [Regex.or.sizeOf_spec]
+
+theorem decreasing_concat_l {α: Type} {σ: Type} [SizeOf σ] (r1 r2: Regex σ) (xs: Hedge α):
+  Prod.Lex
+    (fun a₁ a₂ => sizeOf a₁ < sizeOf a₂)
+    (fun a₁ a₂ => sizeOf a₁ < sizeOf a₂)
+    (xs, r1)
+    (xs, Regex.concat r1 r2) := by
+  apply Prod.Lex.right
+  simp +arith only [Regex.concat.sizeOf_spec]
+
+theorem decreasing_concat_r {α: Type} {σ: Type} [SizeOf σ] (r1 r2: Regex σ) (xs: Hedge α):
+  Prod.Lex
+    (fun a₁ a₂ => sizeOf a₁ < sizeOf a₂)
+    (fun a₁ a₂ => sizeOf a₁ < sizeOf a₂)
+    (xs, r2)
+    (xs, Regex.concat r1 r2) := by
+  apply Prod.Lex.right
+  simp +arith only [Regex.concat.sizeOf_spec]
+
+theorem decreasing_star {α: Type} {σ: Type} [SizeOf σ] (r: Regex σ) (xs: Hedge α):
+  Prod.Lex
+    (fun a₁ a₂ => sizeOf a₁ < sizeOf a₂)
+    (fun a₁ a₂ => sizeOf a₁ < sizeOf a₂)
+    (xs, r)
+    (xs, Regex.star r) := by
+  apply Prod.Lex.right
+  simp +arith only [Regex.star.sizeOf_spec]
+
+theorem decreasing_symbol {α: Type} {σ: Type} [SizeOf σ] (r1 r2: Regex σ) (x: Hedge.Node α):
+  Prod.Lex
+    (fun a₁ a₂ => sizeOf a₁ < sizeOf a₂)
+    (fun a₁ a₂ => sizeOf a₁ < sizeOf a₂)
+    (x.getChildren, r1)
+    ([x], r2) := by
+  apply Prod.Lex.left
+  cases x with
+  | mk label children =>
+  simp only [Hedge.Node.getChildren]
+  simp only [List.cons.sizeOf_spec, Node.mk.sizeOf_spec, sizeOf_default, add_zero,
+    List.nil.sizeOf_spec]
+  omega
+
+theorem denote_elem_sizeOf_concat_left {α: Type} {σ: Type} [SizeOf σ] {r1 r2: Regex σ} {xs: Hedge α}:
+  Prod.Lex (fun a₁ a₂ => sizeOf a₁ < sizeOf a₂) (fun a₁ a₂ => sizeOf a₁ < sizeOf a₂) (List.take n xs, r1) (xs, Regex.concat r1 r2) := by
+  have h := Hedge.sizeOf_take n xs
+  cases h with
+  | inl h =>
+    rw [h]
+    apply decreasing_concat_l
+  | inr h =>
+    apply Prod.Lex.left
+    assumption
+
+theorem denote_elem_sizeOf_concat_right {α: Type} {σ: Type} [SizeOf σ] {p q: Regex σ} {xs: Hedge α}:
+  Prod.Lex (fun a₁ a₂ => sizeOf a₁ < sizeOf a₂) (fun a₁ a₂ => sizeOf a₁ < sizeOf a₂) ((List.drop n xs), q) (xs, Regex.concat p q) := by
+  have h := Hedge.sizeOf_drop n xs
+  cases h with
+  | inl h =>
+    rw [h]
+    apply decreasing_concat_r
+  | inr h =>
+    apply Prod.Lex.left
+    assumption
+
+theorem denote_elem_sizeOf_star_left {α: Type} {σ: Type} [SizeOf σ] {p: Regex σ} {xs: Hedge α}:
+  Prod.Lex (fun a₁ a₂ => sizeOf a₁ < sizeOf a₂) (fun a₁ a₂ => sizeOf a₁ < sizeOf a₂) ((List.take n xs), p) (xs, Regex.star p) := by
+  have h := Hedge.sizeOf_take n xs
+  cases h with
+  | inl h =>
+    rw [h]
+    apply decreasing_star
+  | inr h =>
+    apply Prod.Lex.left
+    assumption
+
+theorem denote_elem_sizeOf_star_right {α: Type} {σ: Type} [SizeOf σ] {p: Regex σ} {x: Hedge.Node α} {xs: Hedge α}:
+  Prod.Lex (fun a₁ a₂ => sizeOf a₁ < sizeOf a₂) (fun a₁ a₂ => sizeOf a₁ < sizeOf a₂) ((List.drop (n + 1) (x::xs)), Regex.star p) ((x::xs), Regex.star p) := by
+  simp only [List.drop_succ_cons]
+  apply Prod.Lex.left
+  have h := Hedge.sizeOf_drop n xs
+  cases h with
+  | inl h =>
+    rw [h]
+    simp only [List.cons.sizeOf_spec, lt_add_iff_pos_left, add_pos_iff, zero_lt_one, true_or]
+  | inr h =>
+    simp only [List.cons.sizeOf_spec, gt_iff_lt]
+    omega
+
+-- denote_symbol_lift_take and denote_symbol_lift_drop is used by denote_elem to lift
+--   a Φ predicate to work on an element of the original list:
+-- * (denote_symbol: σ -> List.ElemOf xs -> Prop) -> (σ -> List.ElemOf (List.take n xs) -> Prop)
+-- * (denote_symbol: σ -> List.ElemOf xs -> Prop) -> (σ -> List.ElemOf (List.drop n xs) -> Prop)
+-- This works, because take and drop create infixes of a list and an element of an infix is a element.
+-- We need these lifting functions to make the prove that denote_list = Regex.denote possible.
+-- See denote_list_concat_n and denote_list_star_n for the exact detail.
+
+def denote_symbol_lift_take (n: Nat) (Φ: σ -> Hedge.LabelIn xs -> Prop): (σ -> Hedge.LabelIn (List.take n xs) -> Prop) :=
+  fun (s: σ) (y: Hedge.LabelIn (List.take n xs)) =>
+    Φ s (Hedge.LabelIn.mk y.val xs (by apply Hedge.labelin_take_is_labelelem))
+
+def denote_symbol_lift_drop (n: Nat) (Φ: σ -> Hedge.LabelIn xs -> Prop): (σ -> Hedge.LabelIn (List.drop n xs) -> Prop) :=
+  fun (s: σ) (y: Hedge.LabelIn (List.drop n xs)) =>
+    Φ s (Hedge.LabelIn.mk y.val xs (by apply Hedge.labelin_drop_is_labelelem))
+
+def lift_symbol {x: Hedge.Node α}
+  (Φ: φ -> LabelIn [x] -> Prop): (φ -> LabelIn x.getChildren -> Prop) :=
+  fun p hchildren => Φ p (by
+    clear Φ
+    clear p
+    clear φ
+    unfold LabelIn at *
+    cases hchildren with
+    | mk childlabel hchildren' =>
+    refine (Subtype.mk childlabel ?_)
+    cases x with
+    | mk label children =>
+    simp only [Node.getChildren] at *
+    unfold Hedge.LabelElem
+    simp only [List.flatMap]
+    simp only [List.map, List.flatten]
+    simp only [List.append_eq, List.append_nil]
+    simp only [Node.getLabels]
+    -- aesop?
+    simp_all only [List.mem_flatMap, List.mem_cons, or_true]
+  )
+
+-- denote_elem is an alternative version of Regex.denote that is later proven to be equivalent definitions.
+-- The difference is that the denote_symbol function now has a relationship with the original input list, List.InfixOf.
+-- This relationship is used for proving termination of regular expressions on trees.
+-- The only other changes is that denote_elem contains unfolded versions of Language.or, Language.concat_n and Language.star_n.
+def denote_elem
+  {α: Type} {φ: Type}
+  (G: Hedge.Grammar n φ)
+  (r: Hedge.Grammar.Rule n φ) (xs: Hedge α)
+  (Φ: φ -> Hedge.LabelIn xs -> Prop): Prop :=
+  match r with
+  | Regex.emptyset => Regex.Language.emptyset xs
+  | Regex.emptystr => Regex.Language.emptystr xs
+  | Regex.symbol (pred, ref) =>
+    match xs with
+    | [x] =>
+      (Φ pred (Hedge.LabelIn.self x))
+      /\ denote_elem G (G.lookup ref) x.getChildren (lift_symbol Φ)
+    | _ => False
+  | Regex.or r1 r2 =>
+       (denote_elem G r1 xs Φ)
+    \/ (denote_elem G r2 xs Φ)
+  | Regex.concat r1 r2 =>
+     ∃ (i: Fin (xs.length + 1)),
+       (denote_elem G r1 (List.take i xs) (denote_symbol_lift_take i Φ))
+    /\ (denote_elem G r2 (List.drop i xs) (denote_symbol_lift_drop i Φ))
+  | Regex.star r1 =>
+    match xs with
+    | [] => True
+    | (x'::xs') =>
+       ∃ (i: Fin xs.length),
+         (denote_elem G r1 (List.take (i + 1) (x'::xs')) (denote_symbol_lift_take (i + 1) Φ))
+      /\ (denote_elem G (Regex.star r1) (List.drop (i + 1) (x'::xs')) (denote_symbol_lift_drop (i + 1) Φ))
+  termination_by (xs, r)
+  decreasing_by
+    · apply decreasing_symbol
+    · apply decreasing_or_l
+    · apply decreasing_or_r
+    · apply denote_elem_sizeOf_concat_left
+    · apply denote_elem_sizeOf_concat_right
+    · apply denote_elem_sizeOf_star_left
+    · apply denote_elem_sizeOf_star_right
